src/spec/TLS13.ConnectionState.ProtectedWireLemmas.fsti
@@ -681,6 +681,62 @@ val lemma_server_handshake_install_materials_agree_from_key_schedule
           (CS.record_material_of_traffic_material server_material)
           (CS.record_material_of_traffic_material client_material))
 
+val lemma_server_handshake_write_client_handshake_read_install_aligned_from_key_schedule
+  (server:CS.connection_model)
+  (client:CS.connection_model)
+  (server_material:CS.traffic_key_material)
+  (client_material:CS.traffic_key_material)
+  (server_after:CS.connection_model)
+  (client_after:CS.connection_model)
+  : Lemma
+      (requires
+        (match
+          server.CS.model_handshake.CS.hs_keys.CS.ks_handshake_secret,
+          client.CS.model_handshake.CS.hs_keys.CS.ks_handshake_secret
+        with
+        | Some server_secret, Some client_secret ->
+          Seq.equal server_secret client_secret
+        | _, _ ->
+          False) /\
+        Seq.equal
+          server.CS.model_handshake.CS.hs_transcript
+          client.CS.model_handshake.CS.hs_transcript /\
+        CS.traffic_install_matches_key_schedule_for_role
+          CS.ServerEndpoint
+          server.CS.model_handshake
+          {
+            CS.install_epoch = CS.TrafficHandshake;
+            CS.install_direction = CS.TrafficWrite;
+            CS.install_material = server_material;
+          } /\
+        CS.traffic_install_matches_key_schedule
+          client.CS.model_handshake
+          {
+            CS.install_epoch = CS.TrafficHandshake;
+            CS.install_direction = CS.TrafficRead;
+            CS.install_material = client_material;
+          } /\
+        CS.step_model
+          server
+          (CS.ConnLocalEvent
+            (CS.LocalInstallTrafficKeysForRole {
+              CS.install_role = CS.ServerEndpoint;
+              CS.install_payload = {
+                CS.install_epoch = CS.TrafficHandshake;
+                CS.install_direction = CS.TrafficWrite;
+                CS.install_material = server_material;
+              };
+            })) == Some server_after /\
+        CS.step_model
+          client
+          (CS.ConnLocalEvent
+            (CS.LocalInstallTrafficKeys {
+              CS.install_epoch = CS.TrafficHandshake;
+              CS.install_direction = CS.TrafficRead;
+              CS.install_material = client_material;
+            })) == Some client_after)
+      (ensures write_read_record_material_aligned server_after client_after)
+
 val lemma_client_handshake_write_server_handshake_read_install_aligned
   (client:CS.connection_model)
   (server:CS.connection_model)
@@ -778,6 +834,62 @@ val lemma_client_handshake_install_materials_agree_from_key_schedule
         CS.record_key_iv_material_agrees
           (CS.record_material_of_traffic_material client_material)
           (CS.record_material_of_traffic_material server_material))
+
+val lemma_client_handshake_write_server_handshake_read_install_aligned_from_key_schedule
+  (client:CS.connection_model)
+  (server:CS.connection_model)
+  (client_material:CS.traffic_key_material)
+  (server_material:CS.traffic_key_material)
+  (client_after:CS.connection_model)
+  (server_after:CS.connection_model)
+  : Lemma
+      (requires
+        (match
+          client.CS.model_handshake.CS.hs_keys.CS.ks_handshake_secret,
+          server.CS.model_handshake.CS.hs_keys.CS.ks_handshake_secret
+        with
+        | Some client_secret, Some server_secret ->
+          Seq.equal client_secret server_secret
+        | _, _ ->
+          False) /\
+        Seq.equal
+          client.CS.model_handshake.CS.hs_transcript
+          server.CS.model_handshake.CS.hs_transcript /\
+        CS.traffic_install_matches_key_schedule
+          client.CS.model_handshake
+          {
+            CS.install_epoch = CS.TrafficHandshake;
+            CS.install_direction = CS.TrafficWrite;
+            CS.install_material = client_material;
+          } /\
+        CS.traffic_install_matches_key_schedule_for_role
+          CS.ServerEndpoint
+          server.CS.model_handshake
+          {
+            CS.install_epoch = CS.TrafficHandshake;
+            CS.install_direction = CS.TrafficRead;
+            CS.install_material = server_material;
+          } /\
+        CS.step_model
+          client
+          (CS.ConnLocalEvent
+            (CS.LocalInstallTrafficKeys {
+              CS.install_epoch = CS.TrafficHandshake;
+              CS.install_direction = CS.TrafficWrite;
+              CS.install_material = client_material;
+            })) == Some client_after /\
+        CS.step_model
+          server
+          (CS.ConnLocalEvent
+            (CS.LocalInstallTrafficKeysForRole {
+              CS.install_role = CS.ServerEndpoint;
+              CS.install_payload = {
+                CS.install_epoch = CS.TrafficHandshake;
+                CS.install_direction = CS.TrafficRead;
+                CS.install_material = server_material;
+              };
+            })) == Some server_after)
+      (ensures write_read_record_material_aligned client_after server_after)
 
 val lemma_sent_replay_skip_empty_head_preserves_peer_stream
   (sender:CS.connection_model)
